integrityScript.sml
@@ -751,13 +751,12 @@ val ca_Inv_rebuild_lem = store_thm("ca_Inv_rebuild_lem", ``
     Inv Icoh Icode Icm sc'
 ``,
   RW_TAC std_ss [cm_kernel_po_def] >>
-  IMP_RES_TAC Icm_f_po_def >>
   IMP_RES_TAC cl_wrel_mode_lem >>
   IMP_RES_TAC cl_wrel_exentry_lem >>
   IMP_RES_TAC ca_wrel_mode_lem >>
   IMP_RES_TAC ca_wrel_exentry_lem >>
   FULL_SIMP_TAC std_ss [Inv_lem, Inv_rebuild_po_def] >>
-  METIS_TAC []
+  METIS_TAC [Icm_f_po_def]
 );
 
 (* main bisimulation lemma (assuming proof obligations): 
